testdata/cue/numeric/list_arithmetic_type_error.cue
@@ -1,0 +1,8 @@
+listAdd: [1, 2] + [3, 4]
+listMul: 3 * [1, 2]
+listMul2: [1, 2] * 3
+listSub: [1, 2] - 3
+listDiv: [1, 2] / 3
+structAdd: {a: 1} + {b: 2}
+boolMul: true * false
+nullSub: null - null
