testdata/cue/numeric/string_repeat_multiplication.cue
@@ -1,0 +1,5 @@
+concat:  "a" + "b"
+repeat:  "ab" * 2
+repeatL: 2 * "ab"
+zero:    "xyz" * 0
+strSub:  "a" - "b"
